inductive vect definition

axioms.v
@@ -113,20 +113,35 @@ Hint Rewrite in_map_iff : FunctorInstances.
 
 
 
-Require Import Coq.Vectors.Vector.
+Inductive vect' A : nat -> Type :=
+  | nil' : vect' A 0
+  | cons' : forall (h:A) (n:nat), vect' A n -> vect' A (S n).
 
-Definition vect n t := Vector.t t n.
+Definition vect n t := vect' t n.
 
-Definition vect_map {A B} (f:A->B) {n} (v : vect n A) : vect n B := Vector.map f v.
+Definition vect_map {A B} (f:A->B) : forall {n} (v:vect n A), vect n B :=
+  fix map_fix {n} (v : vect' A n) : vect' B n := match v with
+  | (nil' _) => (nil' _)
+  | (cons' _ a _ v') => cons' _ (f a) _ (map_fix v')
+  end.
+
+Lemma vect_map_id A: forall n (v : vect' A n), vect_map (fun x => x) v = v.
+Proof. induction v. now reflexivity. unfold vect_map in *. rewrite <- IHv. congruence. Defined.
+
+Lemma vect_map_ext A B: forall (f g:A->B), (forall a, f a = g a) -> forall n (v : vect' A n), vect_map f v = vect_map g v.
+Proof. induction v. now reflexivity. unfold vect_map in *. rewrite IHv. congruence. Defined.
+
+Lemma vect_map_map A B C: forall (f:A->B) (g:B->C) n (v : vect' A n), vect_map g (vect_map f v) = vect_map (fun x => g (f x)) v.
+Proof. induction v. now reflexivity. unfold vect_map in *. rewrite IHv. congruence. Defined.
 
 Definition vect_id {A} {f : A -> A} {n} :
   (forall x, f x = x) -> forall (v : vect n A), vect_map f v = v.
-Proof. intros H v. unfold vect_map. rewrite <- Vector.map_id. now apply Vector.map_ext. Defined.
+Proof. intros H v. unfold vect_map. rewrite <- vect_map_id. now apply vect_map_ext. Defined.
 
 Definition vect_ext {A B} {f f' : A -> B} {n} :
   (forall x, f x = f' x) -> forall (v: vect n A), vect_map f v = vect_map f' v.
-Proof. intros H v. unfold vect_map. now apply Vector.map_ext. Defined.
+Proof. intros H v. unfold vect_map. now apply vect_map_ext. Defined.
 
 Definition vect_comp {A B C} {f : A -> B} {g : B -> C} {n} {h} :
   (forall x, (funcomp g f) x =  h x) -> forall (v: vect n _), vect_map g (vect_map f v) = vect_map h v.
-Proof. intros H v. unfold vect_map. rewrite Vector.map_map. apply vect_ext. intro. now rewrite <- H. Defined.
+Proof. intros H v. rewrite vect_map_map. now apply vect_ext. Defined.
